Created an iris Language

.Makefile.d
@@ -1,9 +1,12 @@
-asm.vo asm.glob asm.v.beautified asm.required_vo: asm.v 
-asm.vio: asm.v 
-asm.vos asm.vok asm.required_vos: asm.v 
+AsmGen.vo AsmGen.glob AsmGen.v.beautified AsmGen.required_vo: AsmGen.v CpdtTactics.vo
+AsmGen.vio: AsmGen.v CpdtTactics.vio
+AsmGen.vos AsmGen.vok AsmGen.required_vos: AsmGen.v CpdtTactics.vos
 CpdtTactics.vo CpdtTactics.glob CpdtTactics.v.beautified CpdtTactics.required_vo: CpdtTactics.v 
 CpdtTactics.vio: CpdtTactics.v 
 CpdtTactics.vos CpdtTactics.vok CpdtTactics.required_vos: CpdtTactics.v 
 partial_map.vo partial_map.glob partial_map.v.beautified partial_map.required_vo: partial_map.v 
 partial_map.vio: partial_map.v 
 partial_map.vos partial_map.vok partial_map.required_vos: partial_map.v 
+progLog.vo progLog.glob progLog.v.beautified progLog.required_vo: progLog.v AsmGen.vo
+progLog.vio: progLog.v AsmGen.vio
+progLog.vos progLog.vok progLog.required_vos: progLog.v AsmGen.vos
